refactor: make WfTuple modular

src/NFO/Wff.v
@@ -1,116 +1,13 @@
 (** * NFO.Wff : Well-founded orders on tuples *)
-
-(* begin hide *)
-Require Import Coq.Init.Wf.
-Add LoadPath "src".
+From Internal Require Export WfTuples.
 From NFO Require Import Model.
-From Internal Require Wff2.
-(* end hide *)
 
-(** Variant of Coq.Init.Wf.Fix_F_inv with iff instead of eq *)
-Lemma Fix_F_inv_iff {A} {R: A -> A -> Prop} {Rwf: well_founded R} {F : forall x:A, (forall y:A, R y x -> Prop) -> Prop} : forall (F_ext :
-forall (x:A) (f g:forall y:A, R y x -> Prop),
-  (forall (y:A) (p:R y x), f y p <-> g y p) -> F x f <-> F x g)
-  (x:A) (r s:Acc R x), Fix_F (fun _ => Prop) F r <-> Fix_F (fun _ => Prop) F s.
-Proof.
-intros. induction (Rwf x); intros.
-rewrite <- (Fix_F_eq _ F r); rewrite <- (Fix_F_eq _ F s); intros.
-  apply F_ext; auto.
-Qed.
-
-(** Variant of Coq.Init.Wf.Fix_eq *)
-Lemma Fix_iff {A} {R: A -> A -> Prop} {Rwf: well_founded R} {F : forall x:A, (forall y:A, R y x -> Prop) -> Prop} : forall (F_ext :
-forall (x:A) (f g:forall y:A, R y x -> Prop),
-  (forall (y:A) (p:R y x), f y p <-> g y p) -> F x f <-> F x g) (x:A), Fix Rwf (fun _ => Prop) F x <-> F x (fun (y:A) (p: R y x) => Fix Rwf (fun _ => Prop) F y).
-Proof.
-  intros. unfold Fix.
-  rewrite <- Fix_F_eq.
-  apply F_ext; intros.
-  apply (@Fix_F_inv_iff _ _ Rwf _ F_ext).
-Qed.
-
-(* 
-TODO: use the multiset order extension in https://www21.in.tum.de/~nipkow/misc/multiset.ps
-*)
-
-(** 2 *)
-
-Definition le12 : set -> set * set -> Prop := fun a bs =>
-  match bs with (b1, b2) => a < b1 \/ a < b2 end.
-
-Definition le22 : set * set -> set * set -> Prop := fun a bs =>
-  match a with (a1, a2) => le12 a1 bs /\ le12 a2 bs end.
-Infix "<<" := le22 (at level 50) : type_scope.
-
-Definition list2 {A: Type} := fun x: prod A A => let (x1, x2) := x in 
-  cons x1 (cons x2 nil).
-
-  Require Import Coq.Wellfounded.Transitive_Closure.
-  Require Import Relation_Definitions.
-Require Import Relation_Operators.
-Definition permletrans := (clos_trans _ (Wff2.permle Model.lt)).
-Definition wf_trans: well_founded permletrans.
-Proof.
-  apply wf_clos_trans. apply Wff2.wf_perm. apply wf_lt.
-Qed.
-
-Require Import Coq.Lists.List.
-Require Import Coq.Sorting.Permutation.
-Lemma le2lst:
-  forall x y, x << y -> permletrans (list2 x) (list2 y).
-Proof.
-  intros. destruct x, y. destruct H, H, H0; simpl list2.
-   - apply (t_trans _ _ _ (cons s1 nil)); apply t_step.
-     red. exists (s :: s0 :: nil). split; auto. 
-     pose proof (Wff2.C set Model.lt O (s1 :: nil) (s :: s0 :: nil) ). simpl in H1. auto.
-     exists (s1 :: nil). split; auto. 
-     pose proof (Wff2.C set Model.lt 1 (s1 :: s2 :: nil) nil). simpl in H1. auto.
-  - apply (t_trans _ _ _ (s1 :: s0 :: nil)); apply t_step.
-    red. exists (s :: s0 :: nil). split; auto. 
-    pose proof (Wff2.C set Model.lt O (s1 :: s0 :: nil) (s :: nil) ). simpl in H1. auto.
-    exists (s1 :: s0 :: nil). split; auto. 
-    pose proof (Wff2.C set Model.lt 1 (s1 :: s2 :: nil) (s0 :: nil)). simpl in H1. auto.
-  - apply (t_trans _ _ _ (s0 :: s2 :: nil)); apply t_step.
-  red. exists (s0 :: s :: nil). split. apply perm_swap.
-    pose proof (Wff2.C set Model.lt 1 (s0 :: s2 :: nil) (s :: nil)). simpl in H1. auto.
-    exists (s0 :: s2 :: nil). split; auto. 
-    pose proof (Wff2.C set Model.lt O (s1 :: s2 :: nil) (s0 :: nil) ). simpl in H1. auto.
-  - apply (t_trans _ _ _ (cons s2 nil)); apply t_step.
-    red. exists (s :: s0 :: nil). split; auto. 
-    pose proof (Wff2.C set Model.lt O (s2 :: nil) (s :: s0 :: nil) ). simpl in H1. auto.
-    exists (s2 :: nil). split; auto. 
-    pose proof (Wff2.C set Model.lt 0 (s1 :: s2 :: nil) nil). simpl in H1. auto.
-Qed.
-Require Import Coq.Wellfounded.Inclusion.
-Require Import Coq.Wellfounded.Inverse_Image.
-Require Import Coq.Wellfounded.Transitive_Closure.
-
-Theorem wf_two: well_founded le22.
-Proof.
-  apply (wf_incl _ _ (fun x y => permletrans (list2 x) (list2 y))).
-  unfold inclusion. apply le2lst.
-  apply (wf_inverse_image _ _ (permletrans) list2).
-  apply wf_clos_trans.
-  apply Wff2.wf_perm.
-  apply wf_lt.
-Qed.
-
-Lemma wf_two_ind: forall P : set -> set -> Prop,
-  (forall x1 x2,
-    (forall y1 y2, (y1, y2) << (x1, x2) -> P y1 y2) -> P x1 x2)
-      -> forall x y, P x y.
-Proof.
-  intros P H.
-  cut (forall z, match z with (z1, z2) => P z1 z2 end).
-  - intros. apply (H0 (x, y)).
-  - apply (well_founded_ind wf_two).
-    destruct x. intros. apply (H s s0). intros.
-    apply (H0 (y1, y2)). assumption.
-Qed.
+Infix "<<" := (le22 lt) (at level 50) : type_scope.
+Infix "<<<" := (le33 lt) (at level 50) : type_scope.
 
 (* begin hide *)
 Ltac auto2 := unfold le22; unfold le12; tauto.
-Lemma AA {a a' b b'}: a < a' -> b < a' -> (a, b) << (a', b').
+Lemma AA {a a' b b': set}: a < a' -> b < a' -> (a, b) << (a', b').
 Proof. auto2. Qed. Hint Resolve AA : Wff.
 Lemma AB {a a' b b'}: a < a' -> b < b' -> (a, b) << (a', b').
 Proof. auto2. Qed. Hint Resolve AB : Wff.
@@ -120,45 +17,6 @@ Lemma BB {a a' b b'}: a < b' -> b < b' -> (a, b) << (a', b').
 Proof. auto2. Qed. Hint Resolve BB : Wff.
 (* end hide *)
 
-(** 3 *)
-
-Definition le13 : set -> set * set * set -> Prop := fun a bs =>
-  match bs with (b1, b2, b3) => a < b1 \/ a < b2 \/ a < b3 end.
-
-Definition le33 : set * set * set -> set * set * set -> Prop := fun a bs =>
-  match a with (a1, a2, a3) => le13 a1 bs /\ le13 a2 bs /\ le13 a3 bs end.
-Infix "<<<" := le33 (at level 50) : type_scope.
-
-Definition list3 {A: Type} := fun x : A *A *A=> 
-  match x with (x1, x2, x3) =>
-  x1 :: x2 :: x3 :: nil end.
-
-Axiom le3lst:
-  forall x y, x <<< y -> permletrans (list3 x) (list3 y).
-
-Theorem wf_three: well_founded le33.
-Proof.
-  apply (wf_incl _ _ (fun x y => permletrans (list3 x) (list3 y))).
-  unfold inclusion. apply le3lst.
-  apply (wf_inverse_image _ _ (permletrans) list3).
-  apply wf_clos_trans.
-  apply Wff2.wf_perm.
-  apply wf_lt.
-Qed.
-
-Lemma wf_three_ind:
-  forall P : set -> set -> set -> Prop,
-  (forall x1 x2 x3,
-    (forall y1 y2 y3, (y1, y2, y3) <<< (x1, x2, x3) -> P y1 y2 y3) -> P x1 x2 x3)
-    -> forall x y z : set, P x y z.
-Proof.
-  intros P H.
-  cut (forall a, match a with (a1, a2, a3) => P a1 a2 a3 end).
-  - intros. apply (H0 (x, y, z)).
-  - apply (well_founded_ind wf_three).
-    intros. destruct x, p. apply (H s0 s1 s). intros.
-    apply (H0 (y1, y2, y3)). assumption.
-Qed.
 
 (* begin hide *)
 Ltac auto3 := unfold le33; unfold le13; tauto.
