src/Internal/WfTuples.v
@@ -1,0 +1,180 @@
+(* begin hide *)
+Require Import Coq.Init.Wf.
+Require Import Coq.Wellfounded.Inclusion.
+Require Import Coq.Wellfounded.Inverse_Image.
+Require Import Coq.Wellfounded.Transitive_Closure.
+Require Import Coq.Wellfounded.Transitive_Closure.
+  Require Import Relation_Definitions.
+Require Import Relation_Operators.
+Require Import Coq.Lists.List.
+Require Import Coq.Sorting.Permutation.
+
+Add LoadPath "src".
+(* From NFO Require Import Model. *)
+From Internal Require Wff2.
+(* end hide *)
+
+Section MultiWf.
+
+(** Variant of Coq.Init.Wf.Fix_F_inv with iff instead of eq *)
+Lemma Fix_F_inv_iff {A} {R: A -> A -> Prop} {Rwf: well_founded R} {F : forall x:A, (forall y:A, R y x -> Prop) -> Prop} : forall (F_ext :
+forall (x:A) (f g:forall y:A, R y x -> Prop),
+  (forall (y:A) (p:R y x), f y p <-> g y p) -> F x f <-> F x g)
+  (x:A) (r s:Acc R x), Fix_F (fun _ => Prop) F r <-> Fix_F (fun _ => Prop) F s.
+Proof.
+intros. induction (Rwf x); intros.
+rewrite <- (Fix_F_eq _ F r); rewrite <- (Fix_F_eq _ F s); intros.
+  apply F_ext; auto.
+Qed.
+
+(** Variant of Coq.Init.Wf.Fix_eq *)
+Lemma Fix_iff {A} {R: A -> A -> Prop} {Rwf: well_founded R} {F : forall x:A, (forall y:A, R y x -> Prop) -> Prop} : forall (F_ext :
+forall (x:A) (f g:forall y:A, R y x -> Prop),
+  (forall (y:A) (p:R y x), f y p <-> g y p) -> F x f <-> F x g) (x:A), Fix Rwf (fun _ => Prop) F x <-> F x (fun (y:A) (p: R y x) => Fix Rwf (fun _ => Prop) F y).
+Proof.
+  intros. unfold Fix.
+  rewrite <- Fix_F_eq.
+  apply F_ext; intros.
+  apply (@Fix_F_inv_iff _ _ Rwf _ F_ext).
+Qed.
+
+(* 
+TODO: use the multiset order extension in https://www21.in.tum.de/~nipkow/misc/multiset.ps
+*)
+
+Variable A: Type.
+Variable lt: A -> A -> Prop.
+Variable wf_lt: well_founded lt.
+Local Infix "<" := lt.
+
+(** 2 *)
+
+Definition le12 : A -> A * A -> Prop := fun a bs =>
+  match bs with (b1, b2) => a < b1 \/ a < b2 end.
+
+Definition le22 : A * A -> A * A -> Prop := fun a bs =>
+  match a with (a1, a2) => le12 a1 bs /\ le12 a2 bs end.
+Local Infix "<<" := le22 (at level 50).
+
+Definition list2 {A: Type} := fun x: prod A A => let (x1, x2) := x in 
+  cons x1 (cons x2 nil).
+
+  
+Definition permletrans := (clos_trans _ (Wff2.permle lt)).
+Definition wf_trans: well_founded permletrans.
+Proof.
+  apply wf_clos_trans. apply Wff2.wf_perm. apply wf_lt.
+Qed.
+
+
+Lemma le2lst:
+  forall x y, x << y -> permletrans (list2 x) (list2 y).
+Proof.
+  intros. destruct x, y. destruct H, H, H0; simpl list2.
+   - apply (t_trans _ _ _ (cons a1 nil)); apply t_step.
+     red. exists (a :: a0 :: nil). split; auto. 
+     pose proof (Wff2.C _ lt O (a1 :: nil) (a :: a0 :: nil) ). simpl in H1. auto.
+     exists (a1 :: nil). split; auto. 
+     pose proof (Wff2.C _ lt 1 (a1 :: a2 :: nil) nil). simpl in H1. auto.
+  - apply (t_trans _ _ _ (a1 :: a0 :: nil)); apply t_step.
+    red. exists (a :: a0 :: nil). split; auto. 
+    pose proof (Wff2.C _ lt O (a1 :: a0 :: nil) (a :: nil) ). simpl in H1. auto.
+    exists (a1 :: a0 :: nil). split; auto. 
+    pose proof (Wff2.C _ lt 1 (a1 :: a2 :: nil) (a0 :: nil)). simpl in H1. auto.
+  - apply (t_trans _ _ _ (a0 :: a2 :: nil)); apply t_step.
+    red. exists (a0 :: a :: nil). split. apply perm_swap.
+    pose proof (Wff2.C _ lt 1 (a0 :: a2 :: nil) (a :: nil)). simpl in H1. auto.
+    exists (a0 :: a2 :: nil). split; auto. 
+    pose proof (Wff2.C _ lt O (a1 :: a2 :: nil) (a0 :: nil) ). simpl in H1. auto.
+  - apply (t_trans _ _ _ (a2 :: nil)); apply t_step.
+    red. exists (a :: a0 :: nil). split; auto. 
+    pose proof (Wff2.C _ lt O (a2 :: nil) (a :: a0 :: nil) ). simpl in H1. auto.
+    exists (a2 :: nil). split; auto. 
+    pose proof (Wff2.C _ lt 0 (a1 :: a2 :: nil) nil). simpl in H1. auto.
+Qed.
+
+Theorem wf_two: well_founded le22.
+Proof.
+  apply (wf_incl _ _ (fun x y => permletrans (list2 x) (list2 y))).
+  unfold inclusion. apply le2lst.
+  apply (wf_inverse_image _ _ (permletrans) list2).
+  apply wf_clos_trans.
+  apply Wff2.wf_perm.
+  apply wf_lt.
+Qed.
+
+Lemma wf_two_ind: forall P : A -> A -> Prop,
+  (forall x1 x2,
+    (forall y1 y2, (y1, y2) << (x1, x2) -> P y1 y2) -> P x1 x2)
+      -> forall x y, P x y.
+Proof.
+  intros P H.
+  cut (forall z, match z with (z1, z2) => P z1 z2 end).
+  - intros. apply (H0 (x, y)).
+  - apply (well_founded_ind wf_two).
+    destruct x. intros. apply (H a a0). intros.
+    apply (H0 (y1, y2)). assumption.
+Qed.
+
+(** 3 *)
+
+Definition le13 : A -> A * A * A -> Prop := fun a bs =>
+  match bs with (b1, b2, b3) => a < b1 \/ a < b2 \/ a < b3 end.
+
+Definition le33 : A * A * A -> A * A * A -> Prop := fun a bs =>
+  match a with (a1, a2, a3) => le13 a1 bs /\ le13 a2 bs /\ le13 a3 bs end.
+Local Infix "<<<" := le33 (at level 50).
+
+Definition list3 {A: Type} := fun x : A *A *A=> 
+  match x with (x1, x2, x3) =>
+  x1 :: x2 :: x3 :: nil end.
+
+Lemma le3lst:
+  forall x y, x <<< y -> permletrans (list3 x) (list3 y).
+Proof.
+  intros. destruct x, y, p, p0. destruct H, H, H0, H0, H1; simpl list3.
+  - apply (t_trans _ _ _ (cons a3 nil)).
+  -- apply t_step. red. exists (a1 :: a2 :: a :: nil). split. 
+    reflexivity.
+    pose proof (Wff2.C _ lt O (a3 :: nil) (a1 :: a2 :: a :: nil) ). simpl in H2. auto.
+  -- apply (t_trans _ _ _ (a3 :: a0 :: nil)). apply t_step.
+     exists (a3 :: nil). split; auto. 
+     pose proof (Wff2.C _ lt 1 (a3 :: a0 :: nil) nil). simpl in H2. auto.
+     apply t_step. exists (a3 :: a0 :: nil). split; auto. 
+     pose proof (Wff2.C _ lt 1 (a3 :: a4 :: a0 :: nil) nil). simpl in H2. auto.
+  -
+Admitted.
+
+Theorem wf_three: well_founded le33.
+Proof.
+  apply (wf_incl _ _ (fun x y => permletrans (list3 x) (list3 y))).
+  unfold inclusion. apply le3lst.
+  apply (wf_inverse_image _ _ (permletrans) list3).
+  apply wf_clos_trans.
+  apply Wff2.wf_perm.
+  apply wf_lt.
+Qed.
+
+Lemma wf_three_ind:
+  forall P : A -> A -> A -> Prop,
+  (forall x1 x2 x3,
+    (forall y1 y2 y3, (y1, y2, y3) <<< (x1, x2, x3) -> P y1 y2 y3) -> P x1 x2 x3)
+    -> forall x y z, P x y z.
+Proof.
+  intros P H.
+  cut (forall a, match a with (a1, a2, a3) => P a1 a2 a3 end).
+  - intros. apply (H0 (x, y, z)).
+  - apply (well_founded_ind wf_three).
+    intros. destruct x, p. apply (H a0 a1 a). intros.
+    apply (H0 (y1, y2, y3)). assumption.
+Qed.
+
+
+End MultiWf.
+
+Arguments le22 : default implicits.
+Arguments le33 : default implicits.
+Arguments wf_two : default implicits.
+Arguments wf_three : default implicits.
+Arguments wf_two_ind : default implicits.
+Arguments wf_three_ind : default implicits.
