src/NFO/Morphs.v
@@ -60,7 +60,7 @@ Lemma iin_respects_eeq: forall z x y, eeq x y ->
   /\ (iin x z <-> iin y z).
 Proof.
   induction z.
-  apply (wf_two_ind (fun x y => eeq x y -> _: Prop)).
+  apply (wf_two_ind wf_lt (fun x y => eeq x y -> _: Prop)).
   destruct x1, x2. intros. repeat rewrite iin_unfold. split; apply xor_iff.
   - apply Aeq_Ain. rewrite eeq_unfold in H2; destruct H2. assumption.
   - rewrite eeq_unfold in H2; destruct H2. 
