Makefile
@@ -14,7 +14,7 @@ remake: clean all
 
 coq: coq-common coq-nf2 coq-nfo
 
-coq-common: src/Internal/Wff2.vos src/Internal/Aux.vos src/Internal/FunExt.vos
+coq-common: src/Internal/Wff2.vos src/Internal/WfTuples.vos src/Internal/Aux.vos src/Internal/FunExt.vos
 coq-nf2: src/NF2/Model.vos src/NF2/Ext.vos src/NF2/Sets.vos src/NF2/ZF.vos src/NF2/Classp.vos
 coq-nfo : src/NFO/Xor.vos src/NFO/BoolExpr.vos src/NFO/Model.vos src/NFO/Wff.vos src/NFO/Eeq.vos src/NFO/Iin.vos src/NFO/Morphs.vos src/NFO/Sets.vos src/NFO/Ext.vos src/NFO/Union.vos src/NFO/Main.vos
 
